ReducibilityLetTermRules.v
@@ -105,7 +105,7 @@ Proof.
 
   eapply reducible_let_rule;
    repeat step || top_level_unfold || t_values_info2 || t_deterministic_star || t_termlist || t_instantiate_sat4;
-      eauto with bwf; eauto using subset_same with bfv;
+      unshelve eauto with bwf; eauto using subset_same with bfv;
         eauto with berased.
   - unshelve epose proof (H15 theta ((p, uu) :: (x,t') :: lterms) _ _); tac1;
       eauto 3 using equivalent_sym with b_equiv;
@@ -181,7 +181,7 @@ Proof.
 
   eapply reducible_let2_rule;
    repeat step || top_level_unfold || t_values_info2 || t_deterministic_star || t_termlist || t_instantiate_sat4;
-      eauto with bwf; eauto using subset_same with bfv;
+      unshelve eauto with bwf; eauto using subset_same with bfv;
         eauto with berased.
   - unshelve epose proof (H15 theta ((p, uu) :: (x,t') :: lterms) _ _); tac1;
       eauto 3 using equivalent_sym with b_equiv;
