StrictPositivity.v
@@ -110,4 +110,5 @@ Ltac simp_spos :=
   rewrite strictly_positive_equation_56 in * ||
   rewrite strictly_positive_equation_57 in * ||
   rewrite strictly_positive_equation_58 in * ||
-  rewrite strictly_positive_equation_59.
+  rewrite strictly_positive_equation_59 in * ||
+  rewrite strictly_positive_equation_60.
